frame rule

CSL.v
@@ -19,7 +19,8 @@ Section SeqCSL.
   Definition low_assn (P : assn) : Prop := low_assn E P.
 
   Section Vnotation.
-    Import VectorNotations.
+    Section For_Vector_Notation.
+      Import VectorNotations.
     Hypothesis brr_lowassn : forall (i : nat),
                                (forall tid : Fin.t ntrd, low_assn (fst (bspec i))[@tid]) /\
                                (forall tid : Fin.t ntrd, low_assn (fst (bspec i))[@tid]).
@@ -28,6 +29,7 @@ Section SeqCSL.
     Hypothesis bc_precise :
       forall i (tid : Fin.t ntrd), precise (fst (bspec i))[@tid] /\
                                    precise (snd (bspec i))[@tid].
+    End For_Vector_Notation.
   End Vnotation.
   Variable tid : Fin.t ntrd.
   Definition safe_nt := safe_nt bspec tid.
@@ -69,59 +71,169 @@ Section SeqCSL.
     - exists v; eauto.
   Qed.
 
-  Import Lists.List.ListNotations.
-  Open Scope list_scope.
   Fixpoint writes_var (c : cmd) : list var :=
     match c with
-      | Cskip | Cwrite _ _ | Cbarrier _ => [ ]
-      | Cassign v _ | Cread v _ => v :: []
+      | Cskip | Cwrite _ _ | Cbarrier _ => nil
+      | Cassign v _ | Cread v _ => v :: nil
       | Cseq c1 c2 => writes_var c1 ++ writes_var c2
       | Cif _ c1 c2 => writes_var c1 ++ writes_var c2
       | Cwhile _ c => writes_var c
     end%list.
 
+  Lemma writes_agrees (c1 c2 : cmd) (st1 st2 : state) :
+    c1 / st1 ==>s c2 / st2 ->
+    fst st1 = fst st2 \/
+    exists x v : Z, In x (writes_var c1) /\ fst st2 = upd (fst st1) x v.
+  Proof.
+    induction 1; try (left; now eauto).
+    - destruct IHred as [ ? | [x [ v [Hin Heq] ]] ]; [tauto | right].
+      exists x, v; split; eauto.
+      apply In_app; eauto.
+    - right; exists x, (edenot e s); split; [constructor | subst]; eauto.
+    - right; exists x, v; split; [constructor | subst]; eauto.
+    - left; subst; eauto.
+  Qed.
+
+  Definition inde (R : assn) (ls : list var) :=
+    forall (x : var) (s : stack) (h : pheap) (v : Z),
+      In x ls -> (sat (s, h) R <-> sat ((upd s x v), h) R).
+
+  Lemma writes_agrees' (c1 c2 : cmd) (st1 st2 : state) (h : pheap) (R : assn):
+    c1 / st1 ==>s c2 / st2 ->
+    inde R (writes_var c1) ->
+    sat (fst st1, h) R -> sat (fst st2, h) R.
+  Proof.
+    intros hred hinde hsat; apply writes_agrees in hred as [heq | [x [v [Hin Heq]]]].
+    - rewrite <-heq; eauto.
+    - rewrite Heq; apply hinde; eauto.
+  Qed.
+
+  Lemma writes_inv (c1 c2 : cmd) (st1 st2 : state) :
+    c1 / st1 ==>s c2 / st2 -> forall x, In x (writes_var c2) -> In x (writes_var c1).
+  Proof.
+    induction 1; simpl; eauto.
+    - intros x H'; specialize (IHred x); apply In_app; apply In_app in H'; tauto.
+    - intros x H; apply In_app; tauto.
+    - intros x H; apply In_app; tauto.
+    - intros x H; apply In_app in H; destruct H.
+      + apply In_app in H; tauto.
+      + inversion H.
+  Qed.
+
+  Lemma wait_writes (c1 c2 : cmd) (j : nat) :
+    wait c1 = Some (j, c2) -> forall x, In x (writes_var c2) -> In x (writes_var c1).
+  Proof.
+    revert j c2; induction c1; simpl; try now inversion 1.
+    intros j c2; destruct (wait c1_1) as [[? ?]|]; intros H; inversion H; inversion H2.
+    simpl; intros x H'; apply In_app in H'; apply In_app.
+    specialize (IHc1_1 n c eq_refl x); tauto.
+  Qed.
+
+  Lemma inde_inv1 (c1 c2 : cmd) (st1 st2 : state) (R : assn) :
+    c1 / st1 ==>s c2 / st2 -> inde R (writes_var c1) -> inde R (writes_var c2).
+  Proof.
+    intros H hinde x s h v Hin; specialize (hinde x s h v). 
+    apply (writes_inv H) in Hin; tauto.
+  Qed.
+
+  Lemma inde_inv2 (c1 c2 : cmd) (j : nat) (R : assn) :
+    wait c1 = Some (j, c2) -> inde R (writes_var c1) -> inde R (writes_var c2).
+    intros H hinde x s h v Hin; specialize (hinde x s h v). 
+    apply (wait_writes H) in Hin; tauto.
+  Qed.
+
+  Lemma writes_agrees_mul (c1 c2 : cmd) (st1 st2 : state) (h : pheap) (R : assn):
+    c1 / st1 ==>s* c2 / st2 ->
+    inde R (writes_var c1) ->
+    sat (fst st1, h) R -> sat (fst st2, h) R.
+  Proof.
+    unfold multi_red, multi_red_tup. 
+    remember (c1, st1) as s1; remember (c2, st2) as s2. 
+    cutrewrite (c1 = fst s1); [|subst; eauto]; cutrewrite (st1 = snd s1); [|subst; eauto];
+    cutrewrite (st2 = snd s2); [|subst; eauto].
+    clear c1 c2 st1 st2  Heqs1 Heqs2.
+    induction 1; intros hinde hsat; eauto.
+    destruct x as [c1 st1], y as [c2 st2], z as [c3 st3].
+    unfold red_tup in H.
+    apply IHclos_refl_trans_1n.
+    apply (inde_inv1 H); eauto.
+    apply (writes_agrees' H); eauto.
+  Qed.
+
   Lemma safe_frame : 
     forall (n : nat) (C : cmd) (s : stack) (ph phR : pheap) (Q R : assn) (disR : pdisj ph phR),
-      safe_nt n C s ph Q -> sat (s, phR) R -> 
+      safe_nt n C s ph Q -> sat (s, phR) R -> inde R (writes_var C) ->
       safe_nt n C s (phplus_pheap disR) (Astar Q R).
-    Proof.
-      induction n; intros C s ph phR Q R disR hsafe hsatR; unfold safe_nt; simpl; eauto; 
-      repeat split; unfold safe_nt in hsafe; simpl in *.
-      - intros ?; subst; repeat eexists; eauto.
-        destruct hsafe as [hsafe _]; specialize (hsafe eq_refl);
-        tauto.
-      - intros hf h hdis heq.
-        destruct hsafe as [_ [hsafe _]].
-        assert (pdisj hf phR) as disfh by (apply pdisjC in hdis; apply pdisjE2 in hdis; eauto).
-        assert (pdisj hf ph) as disf by (apply pdisjC in hdis; apply pdisjE1 in hdis; eauto).
-        assert (phplus (phplus ph phR) hf = phplus (phplus ph hf) phR) as heqp.
-        { rewrite <-(phplus_eq disR), phplus_comm; eauto; simpl. 
-          rewrite (phplus_comm disR), padd_left_comm; eauto; 
+  Proof.
+    induction n; intros C s ph phR Q R disR hsafe hsatR hinde; unfold safe_nt; simpl; eauto; 
+    repeat split; unfold safe_nt in hsafe; simpl in *.
+    - intros ?; subst; repeat eexists; eauto.
+      destruct hsafe as [hsafe _]; specialize (hsafe eq_refl);
+      tauto.
+    - intros hf h hdis heq.
+      destruct hsafe as [_ [hsafe _]].
+      assert (pdisj hf phR) as disfh by (apply pdisjC in hdis; apply pdisjE2 in hdis; eauto).
+      assert (pdisj hf ph) as disf by (apply pdisjC in hdis; apply pdisjE1 in hdis; eauto).
+      assert (phplus (phplus ph phR) hf = phplus (phplus ph hf) phR) as heqp.
+      { rewrite <-(phplus_eq disR), phplus_comm; eauto; simpl. 
+        rewrite (phplus_comm disR), padd_left_comm; eauto; 
         [ | rewrite (phplus_comm (pdisjC disR)); eauto].
-          rewrite <-(phplus_eq disf), phplus_comm; simpl; rewrite (@phplus_comm hf ph); eauto.
-          Hint Resolve pdisjC.
-          apply pdisj_padd_expand; eauto; rewrite (@phplus_comm phR ph); eauto. }
-        rewrite heqp, padd_assoc, <-(phplus_eq  disfh) in heq; eauto.
-        assert (pdisj ph (phplus_pheap disfh)) as dis' by (apply pdisj_padd_comm; eauto).
-        apply (hsafe _ _ dis' heq).
-      - apply access_ok_mono; tauto.
-      - apply write_ok_mono; tauto.
-      - intros hF h c' ss' hdis heq hred.
-        assert (phplus (phplus ph phR) hF = phplus ph (phplus phR hF)).
-        { apply padd_assoc; eauto.
-          apply pdisj_padd_expand in hdis; tauto.
-          apply pdisjC in hdis; apply pdisjE2 in hdis; eauto. }
-        destruct hsafe as [_ [_ [_ [_ [hsafe _]]]]].
-        assert (pdisj ph (phplus phR hF)) as hdis'.
-        { apply pdisj_padd_expand in hdis; eauto; tauto. }
-        apply pdisjC in hdis; apply pdisjE2 in hdis; apply pdisjC in hdis.
-        rewrite H, <- (phplus_eq hdis) in heq.
-(*        apply pdisjC, pdisjE1, pdisjC in hdis.*)
-        rewrite <-(phplus_eq hdis) in hdis'.
-        destruct (hsafe _ _ _ _ hdis' heq hred) as  [h' [ph' [? [hdis'' [? ?]]]]]. 
-        assert (pdisj ph' phR) as dis'R by (simpl in hdis''; apply pdisjE1 in hdis''; eauto).
-        assert (pdisj (phplus_pheap dis'R) hF) as dis''' by (simpl; apply pdisj_padd_expand; eauto).
-        exists h', (phplus_pheap dis'R); repeat split; eauto.
-        cutrewrite (phplus (phplus_pheap dis'R) hF = phplus ph' (phplus_pheap hdis));
-          [eauto| apply padd_assoc; eauto].
-        apply IHn; eauto.
+        rewrite <-(phplus_eq disf), phplus_comm; simpl; rewrite (@phplus_comm hf ph); eauto.
+        Hint Resolve pdisjC.
+        apply pdisj_padd_expand; eauto; rewrite (@phplus_comm phR ph); eauto. }
+      rewrite heqp, padd_assoc, <-(phplus_eq  disfh) in heq; eauto.
+      assert (pdisj ph (phplus_pheap disfh)) as dis' by (apply pdisj_padd_comm; eauto).
+      apply (hsafe _ _ dis' heq).
+    - apply access_ok_mono; tauto.
+    - apply write_ok_mono; tauto.
+    - intros hF h c' ss' hdis heq hred.
+      assert (phplus (phplus ph phR) hF = phplus ph (phplus phR hF)).
+      { apply padd_assoc; eauto.
+        apply pdisj_padd_expand in hdis; tauto.
+        apply pdisjC in hdis; apply pdisjE2 in hdis; eauto. }
+      destruct hsafe as [_ [_ [_ [_ [hsafe _]]]]].
+      assert (pdisj ph (phplus phR hF)) as hdis'.
+      { apply pdisj_padd_expand in hdis; eauto; tauto. }
+      apply pdisjC in hdis; apply pdisjE2 in hdis; apply pdisjC in hdis.
+      rewrite H, <- (phplus_eq hdis) in heq.
+      rewrite <-(phplus_eq hdis) in hdis'.
+      destruct (hsafe _ _ _ _ hdis' heq hred) as  [h' [ph' [? [hdis'' [? ?]]]]]. 
+      assert (pdisj ph' phR) as dis'R by (simpl in hdis''; apply pdisjE1 in hdis''; eauto).
+      assert (pdisj (phplus_pheap dis'R) hF) as dis''' by (simpl; apply pdisj_padd_expand; eauto).
+      exists h', (phplus_pheap dis'R); repeat split; eauto.
+      cutrewrite (phplus (phplus_pheap dis'R) hF = phplus ph' (phplus_pheap hdis));
+        [eauto| apply padd_assoc; eauto].
+      apply IHn; eauto.
+      apply (writes_agrees' hred); eauto. apply (inde_inv1 hred); eauto.
+      apply pdisjE1 in hdis'; eauto.
+      apply pdisjC, pdisjE2, pdisjC in hdis; eauto.
+    - destruct hsafe as [_ [_ [_ [_ [_ hsafe]]]]].
+      intros j c' H; destruct (hsafe j c' H) as [phP [ph' [hdisP' [heqP' [Hsat Hq]]]]].
+      assert (pdisj ph' phR) as hdis'R by (rewrite <-heqP' in disR; 
+                                           apply pdisjC, pdisjE2 in disR; eauto).
+      exists phP, (phplus_pheap hdis'R); repeat split; eauto; simpl.
+      apply pdisj_padd_expand; eauto; rewrite <-heqP' in disR; eauto.
+      rewrite <- heqP', padd_assoc; eauto.
+      apply pdisj_padd_expand; eauto; rewrite <-heqP' in disR; eauto.
+      intros phQ H0 Hsatq.
+      assert (pdisj phQ ph') by (apply pdisjE1 in H0; eauto).
+      specialize (Hq phQ H1 Hsatq).
+      assert (pdisj (phplus phQ ph') phR).
+      { apply pdisj_padd_expand; eauto. }
+      cutrewrite (phplus_pheap (h1:=phQ) (h2:=phplus_pheap (h1:=ph') (h2:=phR) hdis'R) H0 = 
+                  phplus_pheap (h1:=phplus_pheap H1) (h2:=phR) H2); 
+        [|apply pheap_eq; simpl; rewrite padd_assoc; eauto].
+      apply IHn; eauto; unfold safe_nt.
+      apply (inde_inv2 H); eauto.
+  Qed.
+  
+  Lemma rule_frame (C : cmd) (P Q R : assn) :
+    CSL P C Q -> inde R (writes_var C) ->
+    CSL (Astar P R) C (Astar Q R).
+  Proof.
+    unfold CSL; intuition. ins. desf. 
+    cutrewrite (ph = phplus_pheap H3); [|destruct ph; apply pheap_eq; eauto].
+    apply safe_frame; eauto.
+  Qed.
+
+End SeqCSL.
